WIP

Strata/Languages/Core/StatementSemantics.lean
@@ -389,6 +389,8 @@ structure WFEvalExtension (φ : CoreEval → Imperative.PureFunc Expression → 
     Imperative.WellFormedSemanticEvalBool (EvalPureFunc φ δ σ decl)
   preserves_wfVal : ∀ δ σ decl, Imperative.WellFormedSemanticEvalVal δ →
     Imperative.WellFormedSemanticEvalVal (EvalPureFunc φ δ σ decl)
+  preserves_wfVar : ∀ δ σ decl, Imperative.WellFormedSemanticEvalVar δ →
+    Imperative.WellFormedSemanticEvalVar (EvalPureFunc φ δ σ decl)
 
 ---------------------------------------------------------------------
 
